theories/Syntax/WeakeningLemmas.v
@@ -236,69 +236,71 @@ Lemma wk_sup {A B a k Γ Δ} (ρ : Δ ≤ Γ) : tSup A⟨ρ⟩ B⟨wk_up A ρ⟩
 Proof. now cbn. Qed.
 
 Lemma wk_elimW {A B P hsup w Γ Δ} (ρ : Δ ≤ Γ)
-  : tWElim A⟨ρ⟩ B⟨wk_up A ρ⟩ P⟨wk_up (tW A⟨ρ⟩ B⟨wk_up A ρ⟩) ρ⟩ hsup⟨ρ⟩ w⟨ρ⟩ = (tWElim A B P hsup w)⟨ρ⟩.
+  : tWElim A⟨ρ⟩ B⟨wk_up A ρ⟩ P⟨wk_up (tW A B) ρ⟩ hsup⟨ρ⟩ w⟨ρ⟩ = (tWElim A B P hsup w)⟨ρ⟩.
 Proof. now cbn. Qed.
 
-(* Definition elimSupHypTy0 A B P :=
+Module ElimSupHypTyDefs.
   (* assuming  Γ ⊢ A,  Γ, a: A ⊢ B and Γ,w : W A B ⊢ P *)
+  Definition ctx0 (Γ : context) (A B P : term) := Γ.
+  Definition argty0 (Γ : context) (A B P : term) := A.
+  Definition ctx1 (Γ : context) (A B P : term) := Γ,,A.
   (* we get Γ, a: A ⊢ B → W A B *)
-  let tyk := arr B ((tW A B)⟨↑⟩) in
-  let ρ := ↑ >> ↑ >> ↑ in
-  let sup := tSup A⟨ρ⟩ B⟨upRen_term_term ρ⟩ (tRel 1) (tRel 0) in
-  tProd B
-   tProd A (tProd tyk (arr (tProd B P)⟨↑ >> ↑⟩ P[sup .: ρ >> tRel])).
-
-Lemma wk_elimSupHypTy {A B P Γ Δ} (ρ : Δ ≤ Γ) :
-  (elimSupHypTy0 A B P)⟨ρ⟩ = elimSupHypTy0 A⟨ρ⟩ B⟨wk_up A ρ⟩ P⟨wk_up (tW A B) ρ⟩.
-Proof.
-  rewrite 2!wk_up_ren_on.
-  unfold elimSupHypTy0.
-  cbn; f_equal; f_equal; f_equal; [f_equal|f_equal|].
-  3: asimpl.
-  all: try reflexivity.
-  - unfold funcomp; cbn. admit.
-  - f_equal; cbn; f_equal.
-  2: admit.
-  f_equal.
-  rewrite scons_eta'.
-  cbn; asimpl.
-  cbn. *)
-
-Definition elimSupHypTy Γ A B P :=
-  (* assuming  Γ ⊢ A,  Γ, a: A ⊢ B and Γ,w : W A B ⊢ P *)
-  (* we get Γ, a: A ⊢ B → W A B *)
-  let tyk := arr B (tW A B)⟨@wk1 Γ A⟩ in
-  let ρ : Γ,,A,,tyk ≤ Γ := wk_step tyk (@wk1 Γ A) in
-  (* Γ,, a: A,, k : B → W A B ⊢ forall (b : B a), P[(k b)/w]*)
-  let ihty :=
+  Definition argty1 (Γ : context) (A B P : term) := arr B (tW A B)⟨@wk1 Γ A⟩.
+  Definition ctx2 (Γ : context) (A B P : term) := Γ,,A,,argty1 Γ A B P.
+  Definition wk2 Γ A B P : ctx2 Γ A B P ≤ ctx0 Γ A B P :=
+    wk_step (argty1 Γ A B P) (@wk1 Γ A).
+  Definition argty2 (Γ : context) (A B P : term) :=
+    let ρ := wk2 Γ A B P in
     let argty := B⟨wk_up A ρ⟩[(tRel 1)..] in
     let rec := tApp (tRel 1) (tRel 0) in
-    tProd argty P⟨wk_up (tW A B) (wk_step argty ρ)⟩[rec..]
-  in
-  let ρ' := wk_step ihty ρ in
-  (* Γ,, a : A,, k :  B → W A B, ih : forall (b : B a), P[(k b)/w]  ⊢ sup A B a k : W A B *)
-  let sup := tSup A⟨ρ'⟩ B⟨wk_up A ρ'⟩ (tRel 2) (tRel 1) in
-  tProd A (tProd tyk (arr ihty P[sup .: ρ' >> tRel])).
+    tProd argty P⟨wk_up (tW A B) (wk_step argty ρ)⟩[rec..].
+  Definition ctx3 (Γ : context) (A B P : term) :=
+    ctx2 Γ A B P,, argty2 Γ A B P.
+
+  (* in ctx2 Γ A B P *)
+  Definition concl (Γ : context) (A B P : term) :=
+    let ρ := wk2 Γ A B P in
+    (* Γ,, a : A,, k :  B → W A B, ih : forall (b : B a), P[(k b)/w]  ⊢ sup A B a k : W A B *)
+    let sup := tSup A⟨ρ⟩ B⟨wk_up A ρ⟩ (tRel 1) (tRel 0) in
+    P⟨wk_up (tW A B) ρ⟩[sup..].
+
+  Create HintDb elimSupHypTy.
+  Hint Unfold ctx0 argty0 ctx1 argty1 ctx2 wk2 argty2 ctx3 concl : elimSupHypTy.
+End ElimSupHypTyDefs.
+
+Export(hints) ElimSupHypTyDefs.
+
+Definition elimSupHypTy Γ A B P :=
+  tProd A
+    (tProd (ElimSupHypTyDefs.argty1 Γ A B P)
+      (arr (ElimSupHypTyDefs.argty2 Γ A B P)
+        (ElimSupHypTyDefs.concl Γ A B P))).
+
+Hint Unfold elimSupHypTy elimSupHypTy0 : elimSupHypTy.
 
 Lemma wk_elimSupHypTy {A B P Γ Δ} (ρ : Δ ≤ Γ) :
   (elimSupHypTy Γ A B P)⟨ρ⟩ = elimSupHypTy Δ A⟨ρ⟩ B⟨wk_up A ρ⟩ P⟨wk_up (tW A B) ρ⟩.
 Proof.
- unfold elimSupHypTy.
- rewrite <-wk_prod; f_equal.
- rewrite <-wk_prod; f_equal.
- 1: now bsimpl.
- rewrite <-wk_arr; f_equal.
- 1: rewrite <-wk_prod; f_equal; now bsimpl.
-bsimpl.
+  autounfold with elimSupHypTy; now rasimpl.
+Qed.
 
- f_equal; f_equal.
- rewrite !wk1_ren_on, !wk_step_ren_on, !wk1_ren.
- rewrite wk1_ren.
- cbn.
- rewrite wk_step_ren.
- cbn -[wk_up wk1 wk_step].
- bsimpl. cbn; asimpl; f_equal.
- f_equal.
+Lemma elimSupHypTy0_ctx Γ A B P :
+  elimSupHypTy0 A B P = elimSupHypTy Γ A B P.
+Proof.
+  autounfold with elimSupHypTy; now rasimpl.
+Qed.
+
+Definition elimWSupRed Γ A B P hsup a k :=
+  let ρ := @wk1 Γ (B[a..]) in
+  tApp (tApp (tApp hsup a) k) (tLambda (B[a..]) (tWElim A⟨ρ⟩ B⟨wk_up A ρ⟩ P⟨wk_up (tW A B) ρ⟩ hsup⟨ρ⟩ (tApp k⟨ρ⟩ (tRel 0)))).
+
+Lemma wk_elimWSupRed {A B P hsup a k Γ Δ} (ρ : Δ ≤ Γ) :
+  elimWSupRed Δ A⟨ρ⟩ B⟨wk_up A ρ⟩ P⟨wk_up (tW A B) ρ⟩ hsup⟨ρ⟩ a⟨ρ⟩ k⟨ρ⟩ = (elimWSupRed Γ A B P hsup a k)⟨ρ⟩.
+Proof. unfold elimWSupRed; now rasimpl. Qed.
+
+Lemma elimWSupRed_ctx Γ A B P hsup a k :
+  elimWSupRed Γ A B P hsup a k = elimWSupRed0 A B P hsup a k.
+Proof. unfold elimWSupRed; now rasimpl. Qed.
 
 
 Lemma wk_step_wk1 {A t Γ Δ} (ρ : Δ ≤ Γ) :  t⟨ρ⟩⟨@wk1 Δ A⟩ = t⟨wk_step A ρ⟩.
